Reorg of Store Update lemmas and definitons.

src/simple-proof/proof/Binding.v
@@ -377,3 +377,66 @@ Lemma var_typing_implies_avar_f: forall G a T,
 Proof.
   introv H; dependent induction H; eauto.
 Qed.
+
+(** * Updating the store *)
+Inductive defs_update : defs -> trm_label -> var -> defs -> Prop :=
+| defs_update_var : forall ds a t x,
+    defs_update (defs_cons ds (def_trm a t)) a x (defs_cons ds (def_trm a (trm_var (avar_f x))))
+| defs_update_push : forall ds d a x ds',
+    defs_update ds a x ds' ->
+    defs_update (defs_cons ds d) a x (defs_cons ds' d).
+
+Definition sto_update (s : sto) (x : var) (a : trm_label) (y : var) (s' : sto) :=
+  ok s /\
+  ok s' /\
+  (dom s) = (dom s') /\
+  (forall z v, z <> x ->
+          binds z v s ->
+          binds z v s') /\
+  exists T ds ds', binds x (val_obj T ds) s /\
+              defs_update ds a y ds' /\
+              binds x (val_obj T ds') s'.
+
+Lemma defs_update_open : forall x ds a y ds',
+    defs_update ds a y ds' ->
+    forall ds1, ds = (open_defs x ds1) ->
+           exists ds1', ds' = (open_defs x ds1').
+Proof.
+  introv H. induction H; intros.
+  - destruct ds1; inversions H.
+    exists (defs_cons ds1 (def_trm a (trm_var (avar_f x0)))).
+    reflexivity.
+  - destruct ds1; inversion H0.
+    pose proof (IHdefs_update _ H2) as [?ds ?].
+    subst ds'. exists (defs_cons ds0 d0).
+    reflexivity.
+Qed.
+
+Lemma defs_update_hasnt: forall ds a x ds' l,
+    defs_update ds a x ds' ->
+    defs_hasnt ds l ->
+    defs_hasnt ds' l.
+Proof.
+  introv H; gen l; induction H; intros.
+  - unfold defs_hasnt; simpl.
+    inversion H; cases_if.
+    auto.
+  - unfold defs_hasnt; simpl.
+    assert (label_of_def d <> l).
+    { inversion H0. cases_if. auto. }
+    cases_if.
+    assert (defs_hasnt ds l).
+    { inversion H0. cases_if. auto. }
+    apply IHdefs_update; auto.
+Qed.
+
+Lemma defs_update_hasnt_inv: forall ds a x ds',
+    defs_update ds a x ds' ->
+    defs_hasnt ds (label_trm a) -> False.
+Proof.
+  introv H. induction H; intros.
+  - inversion H; cases_if; congruence.
+  - assert (defs_hasnt ds (label_trm a)).
+    { inversion H0; cases_if. }
+    auto.
+Qed.
