src/simple-proof/proof/StoreUpdate.v
@@ -1,38 +1,154 @@
+(** printing ⊢#    %\vdash_{\#}%    #&vdash;<sub>&#35;</sub>#     *)
+(** printing ⊢##   %\vdash_{\#\#}%  #&vdash;<sub>&#35&#35</sub>#  *)
+(** printing ⊢##v  %\vdash_{\#\#v}% #&vdash;<sub>&#35&#35v</sub># *)
+(** printing ⊢!    %\vdash_!%       #&vdash;<sub>!</sub>#         *)
+(** remove printing ~ *)
+
+(** This module proves the Lemmas about updated stores *)
+
 Set Implicit Arguments.
 
 Require Import Coq.Program.Equality.
-Require Import LibLN.
-Require Import Definitions.
+Require Import LibLN LibExtra.
+Require Import Definitions Binding
+        RecordAndInertTypes PreciseTyping
+        StronglyTypedStores CanonicalForms.
 
-Inductive defs_update : defs -> trm_label -> var -> defs -> Prop :=
-| defs_update_var : forall ds a t x,
-    defs_update (defs_cons ds (def_trm a t)) a x (defs_cons ds (def_trm a (trm_var (avar_f x))))
-| defs_update_push : forall ds d a x ds',
+
+(** * Store updates *)
+Lemma defs_update_typing: forall G ds U ds' a x T,
     defs_update ds a x ds' ->
-    defs_update (defs_cons ds d) a x (defs_cons ds' d).
-
-Definition sto_update (s : sto) (x : var) (a : trm_label) (y : var) (s' : sto) :=
-  ok s /\
-  ok s' /\
-  (dom s) = (dom s') /\
-  (forall z v, z <> x ->
-          binds z v s ->
-          binds z v s') /\
-  exists T ds ds', binds x (val_obj T ds) s /\
-              defs_update ds a y ds' /\
-              binds x (val_obj T ds') s'.
-
-Lemma defs_update_open : forall x ds a y ds',
-    defs_update ds a y ds' ->
-    forall ds1, ds = (open_defs x ds1) ->
-           exists ds1', ds' = (open_defs x ds1').
+    record_type U ->
+    G /- ds :: U ->
+    record_has U (dec_trm a T T) ->
+    G ⊢ trm_var (avar_f x) : T ->
+    G /- ds' :: U.
 Proof.
-  introv H. induction H; intros.
-  - destruct ds1; inversions H.
-    exists (defs_cons ds1 (def_trm a (trm_var (avar_f x0)))).
-    reflexivity.
-  - destruct ds1; inversion H0.
-    pose proof (IHdefs_update _ H2) as [?ds ?].
-    subst ds'. exists (defs_cons ds0 d0).
-    reflexivity.
+  introv H; gen U T. induction H; intros.
+  - inversions H0. inversions H7.
+    inversions H1. eauto.
+    constructor; eauto.
+    inversions H7.
+    assert (T1 = T) by (eapply (unique_rcd_trm H); eauto); subst.
+    eauto.
+  - inversions H1. inversions H.
+    assert (record_type T0).
+    { destruct H0 as [ls ?H]. inversions H0.
+      exists ls0; auto. }
+    inversion H2; subst T0 U D0.
+    + constructor; eauto using defs_update_hasnt.
+    + inversions H9. inversions H8; simpl in *.
+      exfalso. eapply defs_update_hasnt_inv; eauto.
+Qed.
+
+Lemma sto_update_inert: forall G s s' x y a T,
+    inert G ->
+    strongly_typed G s ->
+    G ⊢ trm_asn (avar_f x) a (avar_f y) : T ->
+    sto_update s x a y s' ->
+    strongly_typed G s'.
+Proof.
+  introv Hin Hst Hty Hsto.
+  remember (trm_asn (avar_f x) a (avar_f y)) as t.
+  induction Hty; inversions Heqt; eauto.
+  pose proof (canonical_forms_obj Hin Hst Hty1) as [?S [?ds [?t [?H [?H ?H]]]]].
+  unfold sto_update in Hsto.
+  destruct Hsto as [?Hoks [?Hoks' [?Hdom [?Hbi [?T [?ds [?ds' [?H [?Hdefup ?Hbis']]]]]]]]].
+  pose proof (binds_functional H2 H) as Hveq; inversions Hveq; clear H.
+  unfold strongly_typed; repeat_split_right; auto.
+  rewrite <- Hdom; apply Hst.
+  destruct Hst as [?H [?H [?H ?H]]].
+  intros. clear IHHty1 IHHty2 H3.
+  pose proof (dom_to_binds H6) as [?T ?H].
+  pose proof (H5 _ H6) as Htyv.
+  rewrite H4 in H6.
+  pose proof (dom_to_binds H6) as [?v ?H].
+  pose proof (defs_update_open x Hdefup ds eq_refl) as [?ds' ?Hds'].
+  destruct (var_decide x0 x).
+  - subst. clear H7.
+    eapply ty_val_obj_s; eauto.
+    + pose proof (var_typ_rcd_to_binds Hin Hty1) as [?S [?T [?Hbi ?H]]].
+      pose proof (binds_functional Hbi0 H3); subst T0; clear Hbi0.
+      inversions Htyv. pose proof (binds_functional H9 H2); congruence.
+      pose proof (binds_functional H2 H9). inversions H10.
+      pose proof (binds_functional H3 H8). congruence.
+    + inversions Htyv. pose proof (binds_functional H8 H2); congruence.
+      pose proof (binds_functional H3 H7); subst; clear H7.
+      pose proof (binds_functional H2 H8). inversions H7.
+      pose proof (var_typ_rcd_to_binds Hin Hty1) as [?S [?T [?Hbi [?Hrh [?H ?H]]]]].
+      pose proof (binds_functional H3 Hbi0). inversions H11.
+      eapply defs_update_typing; eauto.
+      pose proof (binds_inert H3 Hin). inversions H11.
+      apply open_record_type; auto.
+      rewrite H12; auto.
+  - apply (Hbi _ _ n) in H7. rename n into Hneq.
+    clear Hbis' H2 Hdefup.
+    inversions Htyv; eauto.
+Qed.
+
+Lemma defs_update_exists: forall ds a t x,
+  defs_has ds (def_trm a t) ->
+  exists ds', defs_update ds a x ds'.
+Proof.
+  intros ds; induction ds; intros.
+  - inversion H.
+  - inversion H. cases_if.
+    + inversions H1.
+      exists (defs_cons ds (def_trm a (trm_var (avar_f x)))); constructor.
+    + apply (IHds a t x) in H1.
+      destruct H1 as [ds' ?H].
+      exists (defs_cons ds' d). constructor; auto.
+Qed.
+
+Lemma sto_updateable: forall s x U ds a t y,
+    ok s ->
+    binds x (val_obj U (open_defs x ds)) s ->
+    defs_has (open_defs x ds) (def_trm a t) ->
+    exists s' ds',
+      ok s' /\
+      dom s = dom s' /\
+      (forall z v, z <> x ->
+              binds z v s ->
+              binds z v s') /\
+      defs_update (open_defs x ds) a y ds' /\
+      binds x (val_obj U ds') s'.
+Proof.
+  intros s; induction s using env_ind; intros.
+  - exfalso. apply (binds_empty_inv H0).
+  - pose proof (defs_update_exists y H1) as [?ds' ?H].
+    pose proof (binds_push_inv H0) as [[?H ?H] | [?H ?H]]; subst.
+    + exists (s & x ~ val_obj U (ds')) ds'.
+      repeat_split_right; auto.
+      * destruct (ok_push_inv H); auto.
+      * simpl_dom; auto.
+      * intros.
+        pose proof (binds_push_inv H4) as [[?H ?H] | [?H ?H]]; try congruence.
+        auto.
+    + assert (Hoks: ok s) by auto.
+      pose proof (IHs x0 _ _ _ _ y Hoks H4 H1) as
+          [?s' [?ds' [?Hoks' [?Hdeq [?H [?H ?H]]]]]].
+      exists (s' & x ~ v) (ds'0). repeat_split_right; auto.
+      * apply ok_push; auto.
+        pose proof (ok_push_inv H) as [_ ?H].
+        rewrite <- Hdeq; auto.
+      * simpl_dom. rewrite Hdeq; auto.
+      * intros.
+        pose proof (binds_push_inv H9) as [[?H ?H] | [?H ?H]]; subst; auto.
+Qed.
+
+Lemma sto_update_exists: forall G s x y a S T,
+    inert G ->
+    strongly_typed G s ->
+    G ⊢ trm_var (avar_f x) : typ_rcd (dec_trm a S T) ->
+    G ⊢ trm_var (avar_f y) : S ->
+    exists s', sto_update s x a y s'.
+Proof.
+  introv Hin Hst Hty HTy.
+  pose proof (canonical_forms_obj).
+  pose proof (canonical_forms_obj Hin Hst Hty) as [?S [?ds [?t [?Hbi [?Hdef _]]]]].
+  unfold strongly_typed in Hst.
+  destruct Hst as [?H [Hok ?H]].
+  pose proof (sto_updateable ds y Hok Hbi Hdef) as [?s' [?ds' [?H ?H]]]; destruct_all.
+  exists s'; unfold sto_update; repeat_split_right; auto.
+  exists S0 (open_defs x ds) ds'; repeat_split_right; auto.
 Qed.
